Splinter/AllocationsLayer/Compactor.i.dfy
@@ -1,0 +1,105 @@
+// Copyright 2018-2021 VMware, Inc., Microsoft Inc., Carnegie Mellon University, ETH Zurich, and University of Washington
+// SPDX-License-Identifier: BSD-2-Clause
+
+// include "../LikesAU.i.dfy"
+// include "../Journal/MiniAllocator.i.dfy"   // tony: borrowing from Journal for now
+include "../Betree/LinkedBranch.i.dfy"
+include "../Betree/BranchSeq.i.dfy"
+include "../Betree/OffsetMap.i.dfy"
+include "MiniAllocator.i.dfy"
+include "LikesAU.i.dfy"
+
+module CompactorMod
+{
+  import opened LinkedBranchMod
+  import opened BranchSeqMod
+  import opened OffsetMapMod
+  import opened MiniAllocatorMod
+  import opened LikesAUMod
+  import opened GenericDisk
+  import opened Sequences
+
+  type BranchDiskView = LinkedBranchMod.DiskView
+
+// Transitions for each thread state machine, from the persective of the caller:
+  //  Init(compact start), Internal, Commit, Abort
+  datatype CompactThread = CompactThread(
+    // Read-only inputs
+    branchSeq: BranchSeq,
+    offsetMap: OffsetMap,  // filter describing which keys from branchSeq should be preserved in output
+    subdisk: BranchDiskView, // diskview containing exactly the part of the tree we are reading
+    // Mutating outputs
+    miniAllocator: MiniAllocator,
+    output: LinkedBranch // root of the tree that we are building. Everything reachable from here is mini-allocated, disk here should be consistent with mini-allocator
+  )
+  
+  datatype Variables = Variables(
+    threads: seq<CompactThread>
+  )
+  {
+    function Likes() : LikesAU {
+      // Union of output.likes and subdisk.Keys (or traverse disk from branchSeq roots?)
+      NoLikes()  // this is a placeholder
+    }
+  }
+
+  datatype TransitionLabel =
+    | Begin(branchSeq: BranchSeq, offsetMap: OffsetMap, subdisk: BranchDiskView)
+    | Internal(allocs: seq<AU>)
+    | Commit(branchSeq: BranchSeq, offsetMap: OffsetMap, subdisk: BranchDiskView, output: LinkedBranch)
+    | Abort(deallocs: seq<AU>)  // allow us to abandon a compaction (even though in practice this is not necessary, via scheduler magic)
+
+  datatype Step = 
+    | BeginStep()
+    | AllocStep(idx: nat)
+    | BuildStep(idx: nat, addr: Address, newOutput: LinkedBranch)
+    | CommitStep(idx: nat)
+    | AbortStep(idx: nat)
+
+
+  predicate Begin(v: Variables, v': Variables, lbl: TransitionLabel) {
+    && lbl.Begin?
+    && var newThread := CompactThread(
+      lbl.branchSeq, 
+      lbl.offsetMap, 
+      lbl.subdisk, 
+      EmptyMiniAllocator(), 
+      LinkedBranch(GenericDisk.Address(0, 0), EmptyDisk())  //placeholder
+      );
+    && v' == v.(threads := v.threads + [newThread])
+  }
+
+  predicate Alloc(v: Variables, v': Variables, lbl: TransitionLabel, idx:nat) {
+    && lbl.Internal?
+    && var thread := v.threads[idx];
+    && var thread' := thread.(miniAllocator := thread.miniAllocator.AddAUs(Set(lbl.allocs)));
+    && v' == v.(threads := v.threads[ idx := thread'])
+  }
+
+  predicate Build(v: Variables, v': Variables, lbl: TransitionLabel, idx:nat, addr: Address, newOutput: LinkedBranch) {
+    && lbl.Internal?
+    && lbl.allocs == []
+    && var thread := v.threads[idx];
+    && thread.miniAllocator.CanAllocate(addr)
+    && newOutput == thread.output // TODO: This is a placeholder for building the tree
+    && var thread' := thread.(
+      miniAllocator := thread.miniAllocator.Allocate(addr),
+      output := newOutput 
+    );
+    && v' == v.(threads := v.threads[ idx := thread'])
+  }
+
+  predicate Commit(: Variables, v': Variables, lbl: TransitionLabel, idx:nat) {
+    && lbl.Commit?
+    && idx < |v.thread|
+    && var thread := v.threads[idx];
+    && lbl.branchSeq == thread.branchSeq
+    && lbl.offsetMap == thread.offsetMap
+    && lbl.subdisk == thread.subdisk
+    && true // TODO: placeholder for thread.output is done
+    && lbl.output == thread.output
+    // reserved set should be same as output.repr, to mean that I used all the stuff I reserved
+    && thread.miniAllocator.GetAllReserved() == thread.output.Representation()
+    && v'.threads == remove(v.threads, idx)
+  }
+}
